Add a C++ implementation for LinearRegions

lib/Lang/LinearRegion_s.h
@@ -1,0 +1,79 @@
+// Copyright 2018-2021 VMware, Inc., Microsoft Inc., Carnegie Mellon University, ETH Zurich, and University of Washington
+// SPDX-License-Identifier: BSD-2-Clause
+
+#pragma once
+
+namespace LinearRegion {
+  typedef struct {
+    // Empty placeholder since NewRegion and FreeRegion are no-ops
+  } Region;
+}
+
+namespace LinearRegionId_s {
+  // We don't define RegionId type, since the only places it is used
+  // are ghost
+}
+
+namespace LinearRegionRefCell_s {
+  template <typename A>
+  using RefCell = std::shared_ptr<A>;
+}
+
+namespace LinearRegionLoc_s {
+  // We don't define Loc type, since the only places it is used
+  // are ghost
+}
+
+namespace LinearRegion_s {
+  using namespace LinearRegion;
+  using namespace LinearRegionRefCell_s;
+
+  template <typename A>
+  A Read(Region g, RefCell<A> r) {
+    (void)g; // Avoid unused variable warning
+    return *r;
+  }
+
+  template <typename A>
+  A Borrow(Region g, RefCell<A> r) {
+    return Read(g, r);
+  }
+
+  template <typename A>
+  void Write(Region g, RefCell<A> r, A a) {
+    (void)g; // Avoid unused variable warning
+    *r = a;
+  }
+
+  template <typename A>
+  void Swap(Region g, RefCell<A> r, A a) {
+    (void)g; // Avoid unused variable warning
+    A tmp = a;
+    a = *r;
+    *r = tmp;
+  }
+
+  template <typename A>
+  RefCell<A> Alloc(Region g, A a) {
+    (void)g; // Avoid unused variable warning
+    std::shared_ptr<A> ret = std::make_shared<A>();
+    *ret = a;
+    return ret;
+  }
+
+  template <typename A>
+  RefCell<A> AllocLinear(Region g, A a) {
+    return Alloc(g, a);
+  }
+
+  Region NewRegion() {
+    Region ret;
+    return ret;
+  }
+
+  void FreeRegion(Region g) {
+    (void)g; // Avoid unused variable warning
+  }
+
+}
+
