lib/Lang/LinearRegion.s.dfy
@@ -2,48 +2,72 @@
 // SPDX-License-Identifier: BSD-2-Clause
 
 
+module {:extern "LinearRegion"} LinearRegion {
+  type {:extern "predefined"} Region
+}
+
+
+module {:extern "LinearRegionId_s"} LinearRegionId {
+  type {:extern "predefined"} RegionId
+}
+
+module {:extern "LinearRegionRefCell_s"} LinearRegionRefCell {
+  type {:extern "predefined"} RefCell(==)<A>
+}
+
+module {:extern "LinearRegionLoc_s"} LinearRegionLoc {
+  type {:extern "predefined"} Loc
+}
+
+
+
 module {:extern "LinearRegion_s"} LinearRegion_s {
+  import LinearRegion
+  import LinearRegionId
+  import LinearRegionRefCell
+  import LinearRegionLoc
+
+  type Region = LinearRegion.Region
+  type RegionId = LinearRegionId.RegionId
+  type RefCell(==)<A> = LinearRegionRefCell.RefCell<A>
+  type Loc = LinearRegionLoc.Loc
 
   // Regions with ML-style ref cells
 
-  type Region
-  type RegionId
-  type RefCell(==)<A>
-  type Loc
 
-  function Id(g: Region): RegionId
-  function Allocated(g: Region): set<Loc>
-  function RefLoc<A>(r: RefCell<A>): Loc
-  function LocRef<A(00)>(l: Loc): RefCell<A>
+  function {:axiom} Id(g: Region): RegionId
+  function {:axiom} Allocated(g: Region): set<Loc>
+  function {:axiom} RefLoc<A>(r: RefCell<A>): Loc
+  function {:axiom} LocRef<A(00)>(l: Loc): RefCell<A>
 
-  predicate ValidRef(loc: Loc, id: RegionId, is_linear: bool)
+  predicate {:axiom} ValidRef(loc: Loc, id: RegionId, is_linear: bool)
 
-  function Get<A>(g: Region, r: RefCell<A>): A
+  function {:axiom} Get<A>(g: Region, r: RefCell<A>): A
 
-  function Modifies(locs: set<Loc>, g1: Region, g2: Region): (b: bool)
+  function {:axiom} Modifies(locs: set<Loc>, g1: Region, g2: Region): (b: bool)
     ensures b ==> Id(g1) == Id(g2)
     ensures b ==> Allocated(g1) <= Allocated(g2)
 
-  function method Read<A>(shared g: Region, r: RefCell<A>): (a: A)
+  function method {:extern "LinearRegion_s", "Read"} Read<A>(shared g: Region, r: RefCell<A>): (a: A)
     requires ValidRef(RefLoc(r), Id(g), false)
     ensures Get(g, r) == a
 
-  function method Borrow<A>(shared g: Region, r: RefCell<A>): (shared a: A)
+  function method {:extern "LinearRegion_s", "Borrow"} Borrow<A>(shared g: Region, r: RefCell<A>): (shared a: A)
     requires ValidRef(RefLoc(r), Id(g), true)
     ensures Get(g, r) == a
 
-  method Write<A>(linear inout g: Region, r: RefCell<A>, a: A)
+  method {:extern "LinearRegion_s", "Write"} Write<A>(linear inout g: Region, r: RefCell<A>, a: A)
     requires ValidRef(RefLoc(r), Id(old_g), false)
     ensures Get(g, r) == a
     ensures Modifies({RefLoc(r)}, old_g, g)
 
-  method Swap<A>(linear inout g: Region, r: RefCell<A>, linear inout a: A)
+  method {:extern "LinearRegion_s", "Swap"} Swap<A>(linear inout g: Region, r: RefCell<A>, linear inout a: A)
     requires ValidRef(RefLoc(r), Id(old_g), true)
     ensures Get(old_g, r) == a
     ensures Get(g, r) == old_a
     ensures Modifies({RefLoc(r)}, old_g, g)
 
-  method Alloc<A>(linear inout g: Region, a: A) returns(r: RefCell<A>)
+  method {:extern "LinearRegion_s", "Alloc"} Alloc<A>(linear inout g: Region, a: A) returns(r: RefCell<A>)
     ensures ValidRef(RefLoc(r), Id(g), false)
     ensures Get(g, r) == a
     ensures Modifies({}, old_g, g)
@@ -51,21 +75,21 @@ module {:extern "LinearRegion_s"} LinearRegion_s {
     ensures RefLoc(r) in Allocated(g)
 
   // TODO: add destructor
-  method AllocLinear<A>(linear inout g: Region, linear a: A) returns(r: RefCell<A>)
+  method {:extern "LinearRegion_s", "AllocLinear"} AllocLinear<A>(linear inout g: Region, linear a: A) returns(r: RefCell<A>)
     ensures ValidRef(RefLoc(r), Id(g), true)
     ensures Get(g, r) == a
     ensures Modifies({}, old_g, g)
     ensures RefLoc(r) !in Allocated(old_g)
     ensures RefLoc(r) in Allocated(g)
 
-  method NewRegion() returns(linear g: Region)
+  method {:extern "LinearRegion_s", "NewRegion"} NewRegion() returns(linear g: Region)
 
   // Note: freeing the region eliminates the permission to alloc/read/write/swap,
   // but it doesn't immediately free the objects in the region,
   // so if the implementation uses reference counting, you still need to break cycles manually
-  method FreeRegion(linear g: Region)
+  method {:extern "LinearRegion_s", "FreeRegion"} FreeRegion(linear g: Region)
 
-  lemma LemmaModifies()
+  lemma {:axiom} LemmaModifies()
     ensures forall g :: Modifies({}, g, g)
     ensures forall locs1, locs2, g1, g2 ::
       Modifies(locs1, g1, g2) && locs1 <= locs2 ==>
@@ -75,7 +99,7 @@ module {:extern "LinearRegion_s"} LinearRegion_s {
         Modifies(locs1, g1, g2) && Modifies(locs2, g2, g3) && locs3 == locs1 + locs2 ==>
         Modifies(locs3, g1, g3)
 
-  lemma LemmaUnmodified<A(00)>()
+  lemma {:axiom} LemmaUnmodified<A(00)>()
     ensures forall r:RefCell<A> {:trigger RefLoc(r)} :: LocRef(RefLoc(r)) == r
     ensures forall l:Loc {:trigger RefLoc<A>(LocRef(l))} :: RefLoc<A>(LocRef(l)) == l
     ensures
@@ -88,7 +112,7 @@ module {:extern "LinearRegion_s"} LinearRegion_s {
 module Test_LinearRegion_s {
   import opened LinearRegion_s
   datatype Node = Nil | Cons(data: bool, next: RefCell<Node>, prev: RefCell<Node>)
-  method M()
+  method Main()
   {
     linear var g := NewRegion();
     var sentinel := Alloc(inout g, Nil);
